WIP

src/Std/Do/Triple/SpecLemmas.lean
@@ -31,35 +31,73 @@ end Std.Range
 
 namespace List
 
+@[simp, grind =]
+theorem cons_head_tail (h : l ≠ []) : l.head h :: l.tail = l := by
+  induction l with
+  | nil => contradiction
+  | cons ih => simp_all
+
+@[ext]
+structure Cursor {α : Type u} (l : List α) : Type u where
+  «prefix» : List α
+  suffix : List α
+  property : «prefix» ++ suffix = l
+
+def Cursor.current {α} {l : List α} (c : Cursor l) (h : 0 < c.suffix.length := by get_elem_tactic) : α :=
+  c.suffix[0]'(by simp [h])
+
+def Cursor.begin (l : List α) : Cursor l := ⟨[], l, rfl⟩
+def Cursor.end (l : List α) : Cursor l := ⟨l, [], by simp⟩
+
+@[simp, grind =] theorem Cursor.prefix_begin (l : List α) : (Cursor.begin l).prefix = [] := rfl
+@[simp, grind =] theorem Cursor.cur_begin (l : List α) (h : 0 < l.length) : (Cursor.begin l).current h = l[0] := rfl
+@[simp, grind =] theorem Cursor.suffix_begin (l : List α) : (Cursor.begin l).suffix = l := rfl
+@[simp, grind =] theorem Cursor.prefix_end (l : List α) : (Cursor.end l).prefix = l := rfl
+@[simp, grind =] theorem Cursor.suffix_end (l : List α) : (Cursor.end l).suffix = [] := rfl
+theorem Cursor.cast_end (l₁ l₂ : List α) (h : l₁ = l₂) : HEq (Cursor.end l₁) (Cursor.end l₂) := by
+  cases h
+  rfl
+
+def Cursor.tail (s : Cursor l) (h : 0 < s.suffix.length := by get_elem_tactic) : Cursor l :=
+  { «prefix» := s.prefix ++ [s.suffix.head (by simp only [List.ne_nil_iff_length_pos, h])]
+  , suffix := s.suffix.tail
+  , property := by simp [s.property] }
+
+end List
+
+namespace List
+
 @[grind →]
-theorem eq_of_range'_eq_append_cons (h : range' s n step = xs ++ cur :: ys) :
-    cur = s + step * xs.length := by
-  rw [range'_eq_append_iff] at h
+theorem cur_of_range'_eq {c : Cursor l} (h : range' s n step = l) (hlen : 0 < c.suffix.length):
+    c.current = s + step * c.prefix.length := by
+  rw [← c.property, range'_eq_append_iff] at h
   obtain ⟨k, hk, hxs, hcur⟩ := h
-  have h := (range'_eq_cons_iff.mp hcur.symm).1.symm
-  have hk : k = xs.length := by simp_all [length_range']
-  simp only [h, hk, Nat.add_left_cancel_iff]
+  obtain ⟨cur, suff, hcons⟩ := length_pos_iff_exists_cons.mp hlen
+  have h := (range'_eq_cons_iff.mp (hcur.symm.trans hcons)).1.symm
+  have hk : k = c.prefix.length := by simp_all [length_range']
+  simp only [Cursor.current, hcons, h, hk, getElem_cons_zero, Nat.add_left_cancel_iff]
   apply Nat.mul_comm
 
-@[grind →]
-theorem length_of_range'_eq_append_cons (h : range' s n step = xs ++ cur :: ys) :
-    n = xs.length + ys.length + 1 := by
-  have : n = (range' s n step).length := by simp
-  simpa [h] using this
+--@[grind →]
+--theorem length_of_range'_eq_append_cons {c : Cursor l} (h : range' s n step = l) :
+--    n = c.prefix.length + c.suffix.length := by
+--  have : n = (range' s n step).length := by simp
+--  simpa [h, ← c.property] using this
 
 @[grind →]
-theorem mem_of_range'_eq_append_cons (h : range' s n step = xs ++ i :: ys) :
-    i ∈ range' s n step := by simp [h]
+theorem Cursor.mem_of_lt_length_suffix {c : Cursor l} (hlen : 0 < c.suffix.length) :
+    c.current ∈ l := by simp [← c.property, Cursor.current]
 
 @[grind →]
-theorem gt_of_range'_eq_append_cons (h : range' s n step = xs ++ i :: ys) (hstep : 0 < step) (hj : j ∈ xs) :
-    j < i := by
-  obtain ⟨nxs, _, rfl, htail⟩ := range'_eq_append_iff.mp h
-  obtain ⟨rfl, _⟩ := range'_eq_cons_iff.mp htail.symm
-  simp only [mem_range'] at hj
-  obtain ⟨i, _, rfl⟩ := hj
-  apply Nat.add_lt_add_left
-  simp [Nat.mul_comm, *]
+theorem gt_of_range'_eq {c : Cursor l} (h : range' s n step = l) (hlen : 0 < c.suffix.length) (hj : j ∈ c.prefix) :
+    j < c.current := by
+  sorry
+--  obtain ⟨nxs, _, rfl, htail⟩ := range'_eq_append_iff.mp h
+--  obtain ⟨rfl, _⟩ := range'_eq_cons_iff.mp htail.symm
+--  simp only [mem_range'] at hj
+--  obtain ⟨i, _, rfl⟩ := hj
+--  apply Nat.add_lt_add_left
+--  simp [Nat.mul_comm, *]
 
 @[grind →]
 theorem lt_of_range'_eq_append_cons (h : range' s n step = xs ++ i :: ys) (hstep : 0 < step) (hj : j ∈ ys) :
@@ -70,24 +108,6 @@ theorem lt_of_range'_eq_append_cons (h : range' s n step = xs ++ i :: ys) (hstep
   omega
 
 end List
-
-namespace Std.List
-
-@[ext]
-structure Zipper {α : Type u} (l : List α) : Type u where
-  rpref : List α
-  suff : List α
-  property : rpref.reverse ++ suff = l
-
-@[simp]
-abbrev Zipper.pref {α} {l : List α} (s : List.Zipper l) : List α := s.rpref.reverse
-
-abbrev Zipper.begin (l : List α) : Zipper l := ⟨[],l,rfl⟩
-abbrev Zipper.end (l : List α) : Zipper l := ⟨l.reverse,[],by simp⟩
-abbrev Zipper.tail (s : Zipper l) (h : s.suff = hd::tl) : Zipper l :=
-  { rpref := hd::s.rpref, suff := tl, property := by simp [s.property, ←h] }
-
-end Std.List
 
 namespace Std.Do
 
@@ -339,7 +359,7 @@ theorem Spec.tryCatch_ExceptT_lift [WP m ps] [Monad m] [MonadExceptOf ε m] (Q :
 The type of loop invariants used by the specifications of `for ... in ...` loops.
 A loop invariant is a `PostCond` that takes as parameters
 
-* A `List.Zipper xs` representing the iteration state of the loop. It is parameterized by the list
+* A `List.Cursor xs` representing the iteration state of the loop. It is parameterized by the list
   of elements `xs` that the `for` loop iterates over.
 * A state tuple of type `β`, which will be a nesting of `MProd`s representing the elaboration of
   `let mut` variables and early return.
@@ -351,7 +371,7 @@ During the induction step, the invariant holds for a suffix with head element `x
 After running the loop body, the invariant then holds after shifting `x` to the prefix.
 -/
 abbrev Invariant {α : Type u} (xs : List α) (β : Type u) (ps : PostShape) :=
-  PostCond (List.Zipper xs × β) ps
+  PostCond (List.Cursor xs × β) ps
 
 /--
 Helper definition for specifying loop invariants for loops with early return.
@@ -365,20 +385,20 @@ It is `none` as long as there was no early return and `some r` if the loop retur
 
 This function allows to specify different invariants for the loop body depending on whether the loop
 terminated early or not. When there was an early return, the loop has effectively finished, which is
-encoded by the additional `⌜xs.suff = []⌝` assertion in the invariant. This assertion is vital for
+encoded by the additional `⌜xs.suffix = []⌝` assertion in the invariant. This assertion is vital for
 successfully proving the induction step, as it contradicts with the assumption that
-`xs.suff = x::rest` of the inductive hypothesis at the start of the loop body, meaning that users
+`xs.suffix = x::rest` of the inductive hypothesis at the start of the loop body, meaning that users
 won't need to prove anything about the bogus case where the loop has returned early yet takes
 another iteration of the loop body.
 -/
 abbrev Invariant.withEarlyReturn
-  (onContinue : List.Zipper xs → β → Assertion ps)
+  (onContinue : List.Cursor xs → β → Assertion ps)
   (onReturn : γ → β → Assertion ps)
   (onExcept : ExceptConds ps := ExceptConds.false) :
     Invariant xs (MProd (Option γ) β) ps :=
   ⟨fun ⟨xs, x, b⟩ => spred(
         (⌜x = none⌝ ∧ onContinue xs b)
-      ∨ (∃ r, ⌜x = some r⌝ ∧ ⌜xs.suff = []⌝ ∧ onReturn r b)),
+      ∨ (∃ r, ⌜x = some r⌝ ∧ ⌜xs.suffix = []⌝ ∧ onReturn r b)),
    onExcept⟩
 
 @[spec]
@@ -386,32 +406,32 @@ theorem Spec.forIn'_list {α β : Type u}
     [Monad m] [WPMonad m ps]
     {xs : List α} {init : β} {f : (a : α) → a ∈ xs → β → m (ForInStep β)}
     (inv : Invariant xs β ps)
-    (step : ∀ b rpref x (hx : x ∈ xs) suff (h : xs = rpref.reverse ++ x :: suff),
-        ⦃inv.1 (⟨rpref, x::suff, by simp [h]⟩, b)}
-        f x hx b
+    (step : ∀ (c : List.Cursor xs) (h : 0 < c.suffix.length) b,
+        ⦃inv.1 (c, b)}
+        f c.current (List.Cursor.mem_of_lt_length_suffix h) b
         ⦃(fun r => match r with
-                   | .yield b' => inv.1 (⟨x::rpref, suff, by simp [h]⟩, b')
-                   | .done b' => inv.1 (⟨xs.reverse, [], by simp⟩, b'), inv.2)}) :
-    ⦃inv.1 (⟨[], xs, by simp⟩, init)} forIn' xs init f ⦃(fun b => inv.1 (⟨xs.reverse, [], by simp⟩, b), inv.2)} := by
-  suffices h : ∀ rpref suff (h : xs = rpref.reverse ++ suff),
-      ⦃inv.1 (⟨rpref, suff, by simp [h]⟩, init)}
-      forIn' (m:=m) suff init (fun a ha => f a (by simp[h,ha]))
-      ⦃(fun b => inv.1 (⟨xs.reverse, [], by simp [h]⟩, b), inv.2)}
-    from h [] xs rfl
-  intro rpref suff h
-  induction suff generalizing rpref init
-  case nil => apply Triple.pure; simp [h]
-  case cons x suff ih =>
+                   | .yield b' => inv.1 (c.tail, b')
+                   | .done b' => inv.1 (.end xs, b'), inv.2)}) :
+    ⦃inv.1 (.begin xs, init)} forIn' xs init f ⦃(fun b => inv.1 (.end xs, b), inv.2)} := by
+  suffices h : ∀ c,
+      ⦃inv.1 (c, init)}
+      forIn' (m:=m) c.suffix init (fun a ha => f a (by simp [←c.property, ha]))
+      ⦃(fun b => inv.1 (.end xs, b), inv.2)}
+    from h (.begin xs)
+  rintro ⟨pref, suff, h⟩
+  induction suff generalizing pref init
+  case nil => apply Triple.pure; simp at h; cases h.symm; rfl
+  case cons x suffix ih =>
     simp only [List.forIn'_cons]
     apply Triple.bind
-    case hx => exact step init rpref x (by simp[h]) suff h
+    case hx => exact step _ (by simp) init
     case hf =>
       intro r
       split
-      next => apply Triple.pure; simp [h]
+      next => apply Triple.pure; simp
       next b =>
         simp
-        have := @ih b (x::rpref) (by simp [h])
+        have := @ih b (pref ++ [x]) (by simp [h])
         simp at this
         exact this
 
@@ -425,22 +445,22 @@ theorem Spec.forIn'_list_const_inv {α β : Type u}
         f x hx b
         ⦃(fun r => match r with | .yield b' => inv.1 b' | .done b' => inv.1 b', inv.2)}) :
     ⦃inv.1 init} forIn' xs init f ⦃inv} :=
-  Spec.forIn'_list (fun p => inv.1 p.2, inv.2) (fun b _ x hx _ _ => step x hx b)
+  Spec.forIn'_list (fun p => inv.1 p.2, inv.2) (fun c h => step c.current (List.Cursor.mem_of_lt_length_suffix h))
 
 @[spec]
 theorem Spec.forIn_list {α β : Type u}
     [Monad m] [WPMonad m ps]
     {xs : List α} {init : β} {f : α → β → m (ForInStep β)}
     (inv : Invariant xs β ps)
-    (step : ∀ b rpref x suff (h : xs = rpref.reverse ++ x :: suff),
-        ⦃inv.1 (⟨rpref, x::suff, by simp [h]⟩, b)}
-        f x b
+    (step : ∀ (c : List.Cursor xs) (h : 0 < c.suffix.length) b,
+        ⦃inv.1 (c, b)}
+        f c.current b
         ⦃(fun r => match r with
-                   | .yield b' => inv.1 (⟨x::rpref, suff, by simp [h]⟩, b')
-                   | .done b' => inv.1 (⟨xs.reverse, [], by simp⟩, b'), inv.2)}) :
-    ⦃inv.1 (⟨[], xs, by simp⟩, init)} forIn xs init f ⦃(fun b => inv.1 (⟨xs.reverse, [], by simp⟩, b), inv.2)} := by
+                   | .yield b' => inv.1 (c.tail, b')
+                   | .done b' => inv.1 (.end xs, b'), inv.2)}) :
+    ⦃inv.1 (.begin xs, init)} forIn xs init f ⦃(fun b => inv.1 (.end xs, b), inv.2)} := by
   simp only [← forIn'_eq_forIn]
-  exact Spec.forIn'_list inv (fun b rpref x _ suff h => step b rpref x suff h)
+  exact Spec.forIn'_list inv step
 
 -- using the postcondition as a constant invariant:
 theorem Spec.forIn_list_const_inv {α β : Type u}
@@ -452,18 +472,18 @@ theorem Spec.forIn_list_const_inv {α β : Type u}
         f hd b
         ⦃(fun r => match r with | .yield b' => inv.1 b' | .done b' => inv.1 b', inv.2)}) :
     ⦃inv.1 init} forIn xs init f ⦃inv} :=
-  Spec.forIn_list (fun p => inv.1 p.2, inv.2) (fun b _ hd _ _ => step hd b)
+  Spec.forIn_list (fun p => inv.1 p.2, inv.2) (fun c hcur => step c.current)
 
 @[spec]
 theorem Spec.foldlM_list {α β : Type u}
     [Monad m] [WPMonad m ps]
     {xs : List α} {init : β} {f : β → α → m β}
     (inv : Invariant xs β ps)
-    (step : ∀ b rpref x suff (h : xs = rpref.reverse ++ x :: suff),
-        ⦃inv.1 (⟨rpref, x::suff, by simp [h]⟩, b)}
-        f b x
-        ⦃(fun b' => inv.1 (⟨x::rpref, suff, by simp [h]⟩, b'), inv.2)}) :
-    ⦃inv.1 (⟨[], xs, by simp⟩, init)} List.foldlM f init xs ⦃(fun b => inv.1 (⟨xs.reverse, [], by simp⟩, b), inv.2)} := by
+    (step : ∀ (c : List.Cursor xs) (h : 0 < c.suffix.length) b,
+        ⦃inv.1 (c, b)}
+        f b c.current
+        ⦃(fun b' => inv.1 (c.tail, b'), inv.2)}) :
+    ⦃inv.1 (.begin xs, init)} List.foldlM f init xs ⦃(fun b => inv.1 (.end xs, b), inv.2)} := by
   have : xs.foldlM f init = forIn xs init (fun a b => .yield <$> f b a) := by
     simp only [List.forIn_yield_eq_foldlM, id_map']
   rw[this]
@@ -481,35 +501,35 @@ theorem Spec.foldlM_list_const_inv {α β : Type u}
         f b hd
         ⦃(fun b' => inv.1 b', inv.2)}) :
   ⦃inv.1 init} List.foldlM f init xs ⦃inv} :=
-    Spec.foldlM_list (fun p => inv.1 p.2, inv.2) (fun b _ hd _ _ => step hd b)
+    Spec.foldlM_list (fun p => inv.1 p.2, inv.2) (fun c hcur => step c.current)
 
 @[spec]
 theorem Spec.forIn'_range {β : Type} {m : Type → Type v} {ps : PostShape}
     [Monad m] [WPMonad m ps]
     {xs : Std.Range} {init : β} {f : (a : Nat) → a ∈ xs → β → m (ForInStep β)}
     (inv : Invariant xs.toList β ps)
-    (step : ∀ b rpref x (hx : x ∈ xs) suff (h : xs.toList = rpref.reverse ++ x :: suff),
-        ⦃inv.1 (⟨rpref, x::suff, by simp [h]⟩, b)}
-        f x hx b
+    (step : ∀ (c : List.Cursor xs.toList) (h : 0 < c.suffix.length) b,
+        ⦃inv.1 (c, b)}
+        f c.current (Std.Range.mem_of_mem_range' (List.Cursor.mem_of_lt_length_suffix h)) b
         ⦃(fun r => match r with
-                   | .yield b' => inv.1 (⟨x::rpref, suff, by simp [h]⟩, b')
-                   | .done b' => inv.1 (⟨xs.toList.reverse, [], by simp⟩, b'), inv.2)}) :
-    ⦃inv.1 (⟨[], xs.toList, by simp⟩, init)} forIn' xs init f ⦃(fun b => inv.1 (⟨xs.toList.reverse, [], by simp⟩, b), inv.2)} := by
+                   | .yield b' => inv.1 (c.tail, b')
+                   | .done b' => inv.1 (.end xs.toList, b'), inv.2)}) :
+    ⦃inv.1 (.begin xs.toList, init)} forIn' xs init f ⦃(fun b => inv.1 (.end xs.toList, b), inv.2)} := by
   simp only [Std.Range.forIn'_eq_forIn'_range', Std.Range.size, Std.Range.size.eq_1]
-  apply Spec.forIn'_list inv (fun b rpref x hx suff h => step b rpref x (Std.Range.mem_of_mem_range' hx) suff h)
+  apply Spec.forIn'_list inv (fun c hcur b => step c hcur b)
 
 @[spec]
 theorem Spec.forIn_range {β : Type} {m : Type → Type v} {ps : PostShape}
     [Monad m] [WPMonad m ps]
     {xs : Std.Range} {init : β} {f : Nat → β → m (ForInStep β)}
     (inv : Invariant xs.toList β ps)
-    (step : ∀ b rpref x suff (h : xs.toList = rpref.reverse ++ x :: suff),
-        ⦃inv.1 (⟨rpref, x::suff, by simp [h]⟩, b)}
-        f x b
+    (step : ∀ (c : List.Cursor xs.toList) (h : 0 < c.suffix.length) b,
+        ⦃inv.1 (c, b)}
+        f c.current b
         ⦃(fun r => match r with
-                   | .yield b' => inv.1 (⟨x::rpref, suff, by simp [h]⟩, b')
-                   | .done b' => inv.1 (⟨xs.toList.reverse, [], by simp⟩, b'), inv.2)}) :
-    ⦃inv.1 (⟨[], xs.toList, by simp⟩, init)} forIn xs init f ⦃(fun b => inv.1 (⟨xs.toList.reverse, [], by simp⟩, b), inv.2)} := by
+                   | .yield b' => inv.1 (c.tail, b')
+                   | .done b' => inv.1 (.end xs.toList, b'), inv.2)}) :
+    ⦃inv.1 (.begin xs.toList, init)} forIn xs init f ⦃(fun b => inv.1 (.end xs.toList, b), inv.2)} := by
   simp only [Std.Range.forIn_eq_forIn_range', Std.Range.size]
   apply Spec.forIn_list inv step
 
@@ -523,15 +543,15 @@ theorem Spec.forIn'_prange {α β : Type u}
     [LawfulUpwardEnumerableLowerBound sl α] [LawfulUpwardEnumerableUpperBound su α]
     {xs : PRange ⟨sl, su⟩ α} {init : β} {f : (a : α) → a ∈ xs → β → m (ForInStep β)}
     (inv : Invariant xs.toList β ps)
-    (step : ∀ b rpref x (hx : x ∈ xs) suff (h : xs.toList = rpref.reverse ++ x :: suff),
-        ⦃inv.1 (⟨rpref, x::suff, by simp [h]⟩, b)}
-        f x hx b
+    (step : ∀ (c : List.Cursor xs.toList) (h : 0 < c.suffix.length) b,
+        ⦃inv.1 (c, b)}
+        f c.current (by exact mem_toList_iff_mem.mp (List.Cursor.mem_of_lt_length_suffix h)) b
         ⦃(fun r => match r with
-                   | .yield b' => inv.1 (⟨x::rpref, suff, by simp [h]⟩, b')
-                   | .done b' => inv.1 (⟨xs.toList.reverse, [], by simp⟩, b'), inv.2)}) :
-    ⦃inv.1 (⟨[], xs.toList, by simp⟩, init)} forIn' xs init f ⦃(fun b => inv.1 (⟨xs.toList.reverse, [], by simp⟩, b), inv.2)} := by
+                   | .yield b' => inv.1 (c.tail, b')
+                   | .done b' => inv.1 (.end xs.toList, b'), inv.2)}) :
+    ⦃inv.1 (.begin xs.toList, init)} forIn' xs init f ⦃(fun b => inv.1 (.end xs.toList, b), inv.2)} := by
   simp only [forIn'_eq_forIn'_toList]
-  apply Spec.forIn'_list inv (fun b rpref x hx suff h => step b rpref x (mem_toList_iff_mem.mp hx) suff h)
+  apply Spec.forIn'_list inv step
 
 open Std.PRange in
 @[spec]
@@ -543,44 +563,44 @@ theorem Spec.forIn_prange {α β : Type u}
     [LawfulUpwardEnumerableLowerBound sl α] [LawfulUpwardEnumerableUpperBound su α]
     {xs : PRange ⟨sl, su⟩ α} {init : β} {f : α → β → m (ForInStep β)}
     (inv : Invariant xs.toList β ps)
-    (step : ∀ b rpref x suff (h : xs.toList = rpref.reverse ++ x :: suff),
-        ⦃inv.1 (⟨rpref, x::suff, by simp [h]⟩, b)}
-        f x b
+    (step : ∀ (c : List.Cursor xs.toList) (h : 0 < c.suffix.length) b,
+        ⦃inv.1 (c, b)}
+        f c.current b
         ⦃(fun r => match r with
-                   | .yield b' => inv.1 (⟨x::rpref, suff, by simp [h]⟩, b')
-                   | .done b' => inv.1 (⟨xs.toList.reverse, [], by simp⟩, b'), inv.2)}) :
-    ⦃inv.1 (⟨[], xs.toList, by simp⟩, init)} forIn xs init f ⦃(fun b => inv.1 (⟨xs.toList.reverse, [], by simp⟩, b), inv.2)} := by
+                   | .yield b' => inv.1 (c.tail, b')
+                   | .done b' => inv.1 (.end xs.toList, b'), inv.2)}) :
+    ⦃inv.1 (.begin xs.toList, init)} forIn xs init f ⦃(fun b => inv.1 (.end xs.toList, b), inv.2)} := by
   simp only [forIn]
-  apply Spec.forIn'_prange inv (fun b rpref x _hx suff h => step b rpref x suff h)
+  apply Spec.forIn'_prange inv step
 
 @[spec]
 theorem Spec.forIn'_array {α β : Type u}
     [Monad m] [WPMonad m ps]
     {xs : Array α} {init : β} {f : (a : α) → a ∈ xs → β → m (ForInStep β)}
     (inv : Invariant xs.toList β ps)
-    (step : ∀ b rpref x (hx : x ∈ xs) suff (h : xs.toList = rpref.reverse ++ x :: suff),
-        ⦃inv.1 (⟨rpref, x::suff, by simp [h]⟩, b)}
-        f x hx b
+    (step : ∀ (c : List.Cursor xs.toList) (h : 0 < c.suffix.length) b,
+        ⦃inv.1 (c, b)}
+        f c.current (by exact Array.mem_toList_iff.mp (List.Cursor.mem_of_lt_length_suffix h)) b
         ⦃(fun r => match r with
-                   | .yield b' => inv.1 (⟨x::rpref, suff, by simp [h]⟩, b')
-                   | .done b' => inv.1 (⟨xs.toList.reverse, [], by simp⟩, b'), inv.2)}) :
-    ⦃inv.1 (⟨[], xs.toList, by simp⟩, init)} forIn' xs init f ⦃(fun b => inv.1 (⟨xs.toList.reverse, [], by simp⟩, b), inv.2)} := by
+                   | .yield b' => inv.1 (c.tail, b')
+                   | .done b' => inv.1 (.end xs.toList, b'), inv.2)}) :
+    ⦃inv.1 (.begin xs.toList, init)} forIn' xs init f ⦃(fun b => inv.1 (.end xs.toList, b), inv.2)} := by
   cases xs
   simp
-  apply Spec.forIn'_list inv (fun b rpref x hx suff h => step b rpref x (by simp[hx]) suff h)
+  apply Spec.forIn'_list inv step
 
 @[spec]
 theorem Spec.forIn_array {α β : Type u}
     [Monad m] [WPMonad m ps]
     {xs : Array α} {init : β} {f : α → β → m (ForInStep β)}
     (inv : Invariant xs.toList β ps)
-    (step : ∀ b rpref x suff (h : xs.toList = rpref.reverse ++ x :: suff),
-        ⦃inv.1 (⟨rpref, x::suff, by simp [h]⟩, b)}
-        f x b
+    (step : ∀ (c : List.Cursor xs.toList) (h : 0 < c.suffix.length) b,
+        ⦃inv.1 (c, b)}
+        f c.current b
         ⦃(fun r => match r with
-                   | .yield b' => inv.1 (⟨x::rpref, suff, by simp [h]⟩, b')
-                   | .done b' => inv.1 (⟨xs.toList.reverse, [], by simp⟩, b'), inv.2)}) :
-    ⦃inv.1 (⟨[], xs.toList, by simp⟩, init)} forIn xs init f ⦃(fun b => inv.1 (⟨xs.toList.reverse, [], by simp⟩, b), inv.2)} := by
+                   | .yield b' => inv.1 (c.tail, b')
+                   | .done b' => inv.1 (.end xs.toList, b'), inv.2)}) :
+    ⦃inv.1 (.begin xs.toList, init)} forIn xs init f ⦃(fun b => inv.1 (.end xs.toList, b), inv.2)} := by
   cases xs
   simp
   apply Spec.forIn_list inv step
@@ -590,11 +610,11 @@ theorem Spec.foldlM_array {α β : Type u}
     [Monad m] [WPMonad m ps]
     {xs : Array α} {init : β} {f : β → α → m β}
     (inv : Invariant xs.toList β ps)
-    (step : ∀ b rpref x suff (h : xs.toList = rpref.reverse ++ x :: suff),
-        ⦃inv.1 (⟨rpref, x::suff, by simp [h]⟩, b)}
-        f b x
-        ⦃(fun b' => inv.1 (⟨x::rpref, suff, by simp [h]⟩, b'), inv.2)}) :
-    ⦃inv.1 (⟨[], xs.toList, by simp⟩, init)} Array.foldlM f init xs ⦃(fun b => inv.1 (⟨xs.toList.reverse, [], by simp⟩, b), inv.2)} := by
+    (step : ∀ (c : List.Cursor xs.toList) (h : 0 < c.suffix.length) b,
+        ⦃inv.1 (c, b)}
+        f b c.current
+        ⦃(fun b' => inv.1 (c.tail, b'), inv.2)}) :
+    ⦃inv.1 (.begin xs.toList, init)} Array.foldlM f init xs ⦃(fun b => inv.1 (.end xs.toList, b), inv.2)} := by
   cases xs
   simp
   apply Spec.foldlM_list inv step
